CrashTolerantReprJournal draft

Splinter/Betree/ReprBetree.i.dfy
@@ -93,6 +93,12 @@ module ReprBetree
     false
   }
 
+  predicate InternalFlushMemtable(v: Variables, v': Variables, lbl: TransitionLabel, step: Step)
+  {
+    // TODO
+    false
+  }
+
   predicate InternalFlush(v: Variables, v': Variables, lbl: TransitionLabel, step: Step)
   {
     // TODO
@@ -124,6 +130,7 @@ module ReprBetree
       case InternalGrowStep(_) => InternalGrow(v, v', lbl, step)
       case InternalSplitStep(_, _, _, _) => InternalSplit(v, v', lbl, step)
       case InternalFlushStep(_, _, _, _, _) => InternalFlush(v, v', lbl, step)
+      case InternalFlushMemtableStep(_) => InternalFlushMemtable(v, v', lbl, step)
       case InternalCompactStep(_, _, _, _) => InternalCompact(v, v', lbl, step)
     }
   }
