Splinter/BlockLayer/CrashTolerantReprJournal.i.dfy
@@ -1,0 +1,221 @@
+// Copyright 2018-2021 VMware, Inc., Microsoft Inc., Carnegie Mellon University, ETH Zurich, and University of Washington
+// SPDX-License-Identifier: BSD-2-Clause
+
+include "../Journal/ReprJournal.i.dfy"
+include "../Journal/LinkedJournal.i.dfy"
+include "../CoordinationLayer/CrashTolerantJournal.i.dfy"
+
+// TODO(jonh): This is a copy-paste of Splinter/CoordinationSystem/CrashTolerantJournal. Functor-reuse?
+
+module CrashTolerantReprJournal {
+  import opened Options
+  // import opened ValueMessage
+  // import opened KeyType
+  // import opened StampedMod
+  import opened MsgHistoryMod
+  // import opened LSNMod
+  import opened GenericDisk
+  import LinkedJournal
+  import ReprJournal
+  import CrashTolerantJournal
+
+  datatype TransitionLabel = TransitionLabel(allocations: seq<Address>, freed: seq<Address>, base: CrashTolerantJournal.TransitionLabel)
+
+  type StoreImage = LinkedJournal.TruncatedJournal
+
+  datatype Ephemeral =
+    | Unknown
+    | Known(v: ReprJournal.Variables)
+  {
+    predicate WF() {
+      Known? ==> v.WF()
+    }
+  }
+
+  datatype Variables = Variables(
+    persistent: StoreImage,
+    ephemeral: Ephemeral,
+    inFlight: Option<StoreImage>
+  )
+  {
+    predicate WF() {
+      && persistent.WF()
+      && ephemeral.WF()
+      && (inFlight.Some? ==> inFlight.value.WF())
+    }
+
+    // function Repr() : set<Address>
+    // {
+    //   if ephemeral.Known?
+    //   then ephemeral.v.journal.truncatedJournal.Representation()
+    //   else persistent.Representation()
+    // }
+  }
+
+  predicate LoadEphemeralFromPersistent(v: Variables, v': Variables, lbl: TransitionLabel)
+  {
+    // Enabling conditions
+    && v.WF()
+    && lbl.base.LoadEphemeralFromPersistentLabel?
+    && lbl.allocations == []
+    && lbl.freed == []
+    && v.ephemeral.Unknown?
+    && v'.ephemeral.Known?
+    // State update
+    && ReprJournal.Init(v'.ephemeral.v, v.persistent)
+    && v'.persistent == v.persistent // UNCHANGED
+    && v'.inFlight == v.inFlight // UNCHANGED
+  }
+
+  predicate ReadForRecovery(v: Variables, v': Variables, lbl: TransitionLabel)
+  {
+    // Enabling conditions
+    && v.WF()
+    && lbl.base.ReadForRecoveryLabel?
+    && lbl.allocations == []
+    && lbl.freed == []
+    && v.ephemeral.Known?
+    && v'.ephemeral.Known?
+    // State update
+    && ReprJournal.Next(v.ephemeral.v, v'.ephemeral.v, ReprJournal.ReadForRecoveryLabel(lbl.base.records))
+    && v' == v  // everything UNCHANGED
+  }
+
+  predicate QueryEndLsn(v: Variables, v': Variables, lbl: TransitionLabel)
+  {
+    // Enabling conditions
+    && v.WF()
+    && lbl.base.QueryEndLsnLabel?
+    && lbl.allocations == []
+    && lbl.freed == []
+    && v.ephemeral.Known?
+    && v'.ephemeral.Known?
+    // State update
+    && ReprJournal.Next(v.ephemeral.v, v'.ephemeral.v, ReprJournal.QueryEndLsnLabel(lbl.base.endLsn))
+    && v' == v
+  }
+
+  predicate Put(v: Variables, v': Variables, lbl: TransitionLabel)
+  {
+    && v.WF()
+    && lbl.base.PutLabel?
+    && lbl.allocations == []
+    && lbl.freed == []
+    && v.ephemeral.Known?
+    && v'.ephemeral.Known?
+
+    && ReprJournal.Next(v.ephemeral.v, v'.ephemeral.v, ReprJournal.PutLabel(lbl.base.records))
+    && v'.persistent == v.persistent // UNCHANGED
+    && v'.inFlight == v.inFlight // UNCHANGED
+  }
+
+  predicate Internal(v: Variables, v': Variables, lbl: TransitionLabel)
+  {
+    && v.WF()
+    && lbl.base.InternalLabel?
+    && |lbl.allocations| == 1
+    && lbl.freed == []
+    && v.ephemeral.Known?
+    && v'.ephemeral.Known?
+
+    && ReprJournal.Next(v.ephemeral.v, v'.ephemeral.v, ReprJournal.InternalLabel(lbl.allocations[0]))
+    && v'.persistent == v.persistent // UNCHANGED
+    && v'.inFlight == v.inFlight // UNCHANGED
+  }
+
+  predicate QueryLsnPersistence(v: Variables, v': Variables, lbl: TransitionLabel)
+  {
+    && v.WF()
+    && lbl.base.QueryLsnPersistenceLabel?
+    && lbl.allocations == []
+    && lbl.freed == []
+    && lbl.base.syncLsn <= v.persistent.SeqEnd()
+    && v' == v
+  }
+
+  predicate CommitStart(v: Variables, v': Variables, lbl: TransitionLabel)
+  {
+    && v.WF()
+    && lbl.base.CommitStartLabel?
+    && lbl.allocations == []
+    && lbl.freed == []
+    && v.ephemeral.Known?
+    // Can't start a commit if one is in-flight, or we'd forget to maintain the
+    // invariants for the in-flight one.
+    && v.inFlight.None?
+    && v'.ephemeral.Known?
+    && v'.inFlight.Some?
+
+    && var frozenJournal := v'.inFlight.value;
+
+    // Frozen journal stitches to frozen map
+    && frozenJournal.SeqStart() == lbl.base.newBoundaryLsn
+
+    // Journal doesn't go backwards
+    && frozenJournal.WF()
+    && v.persistent.SeqEnd() <= frozenJournal.SeqEnd()
+
+    // There should be no way for the frozen journal to have passed the ephemeral map!
+    && frozenJournal.SeqStart() <= lbl.base.maxLsn
+
+    && ReprJournal.Next(v.ephemeral.v, v'.ephemeral.v, ReprJournal.FreezeForCommitLabel(frozenJournal))
+
+    && v' == v.(
+      ephemeral := v'.ephemeral,  // given by predicate above (but happens to be read-only / unchanged)
+      inFlight := Some(frozenJournal) // given by predicates above
+      )
+  }
+
+  predicate CommitComplete(v: Variables, v': Variables, lbl: TransitionLabel)
+  {
+    && v.WF()
+    && lbl.base.CommitCompleteLabel?
+    && lbl.allocations == []
+    && v.ephemeral.Known?
+    && v.inFlight.Some?
+    && v'.ephemeral.Known?
+
+    && ReprJournal.Next(v.ephemeral.v, v'.ephemeral.v,
+        ReprJournal.DiscardOldLabel(v.inFlight.value.SeqStart(), lbl.base.requireEnd, lbl.freed))
+
+    && v' == v.(
+      persistent := v.inFlight.value,
+      ephemeral := v'.ephemeral,  // given by predicate above
+      inFlight := None)
+  }
+
+  predicate Crash(v: Variables, v': Variables, lbl: TransitionLabel)
+  {
+    && v.WF()
+    && lbl.base.CrashLabel?
+    && lbl.allocations == []
+    && lbl.freed == []
+    && v' == v.(
+      ephemeral := Unknown,
+      inFlight := None)
+  }
+
+  // Models mkfs
+  predicate Init(v: Variables)
+  {
+    v == Variables(LinkedJournal.Mkfs(), Unknown, None)
+  }
+
+  predicate Next(v: Variables, v': Variables, lbl: TransitionLabel)
+  {
+    match lbl.base {
+      case LoadEphemeralFromPersistentLabel() => LoadEphemeralFromPersistent(v, v', lbl)
+      case ReadForRecoveryLabel(_) => ReadForRecovery(v, v', lbl)
+      case QueryEndLsnLabel(_) => QueryEndLsn(v, v', lbl)
+      case PutLabel(_) => Put(v, v', lbl)
+      case InternalLabel() => Internal(v, v', lbl)
+      case QueryLsnPersistenceLabel(_) => QueryLsnPersistence(v, v', lbl)
+      case CommitStartLabel(_, _) => CommitStart(v, v', lbl)
+      case CommitCompleteLabel(_) => CommitComplete(v, v', lbl)
+      case CrashLabel() => Crash(v, v', lbl)
+    }
+  }
+
+
+}
+
